src/tosmt/term.fsi
@@ -129,6 +129,7 @@ val declToSmt: string -> decl -> string
 val mk_Kind_type : term
 val mk_Typ_app : term -> term -> term
 val mk_Typ_dep : term -> term -> term
+val mk_Typ_uvar: int -> term
 val mk_and_l: list<term> -> term
 val mk_or_l: list<term> -> term
 
